proving soundness

FY/Assertion.v
@@ -23,11 +23,8 @@ Definition pre_init (n: nat) (m: Unitary (2^n))
 Definition init_sub (n: nat) (P : Assertion n) : Assertion (n - 1) := 
     pair (StateOf P) (pair (PropOf P) (pre_init n (DensityOf P))).
 
-Definition apply_sub n (U: Unitary (2^n)) (P : Assertion n) : Assertion n :=
-  pair (StateOf P) (pair (PropOf P) (U† × (DensityOf P) × U)). 
-
-Definition AssertionWithDensity (n m: nat) (P: Assertion n) (U: Unitary (2^m)) : Assertion m := 
-  (StateOf P, (PropOf P, U)).
+Definition apply_sub n m (U: Unitary (2^n)) (P : Assertion n) : Assertion n :=
+  pair (StateOf P) (pair (PropOf P) ((padding n m U)† × (DensityOf P) × (padding n m U))). 
 
 Definition AssertionOf (n: nat) (st: total_map nat) 
 (prop: bool_exp) (U: Unitary (2^n)) : Assertion n := 
