FY/Soundness.v
@@ -7,38 +7,65 @@ From FY Require Export Semantics.
 From FY Require Export Assertion.
 From FY Require Export Logic.
 
-Inductive derivable (np nq: nat) : Assertion np -> com -> Assertion nq -> Type :=
-| H_Skip : forall P,
-    derivable P <{skip}> P
-| H_Asgn : forall Q V a,
-    derivable (Q [V ⊢> a]) <{X := a}> Q
-| H_Seq : forall P c Q d R,
-    derivable P c Q -> derivable Q d R -> derivable P <{c;d}> R
-| H_If : forall P Q b c1 c2,
-  derivable (fun st => P st ∧ bassn b st) c1 Q ->
-  derivable (fun st => P st ∧ ~(bassn b st)) c2 Q ->
-  derivable P <{if b then c1 else c2 end}> Q
-| H_While : forall P b c,
-  derivable (fun st => P st ∧ bassn b st) c P ->
-  derivable P <{while b do c end}> (fun st => P st ∧ ~ (bassn b st))
-| H_Consequence : forall (P Q P' Q' : Assertion) c,
-  derivable P' c Q' ->
-  (forall st, P st -> P' st) ->
-  (forall st, Q' st -> Q st) ->
-  derivable P c Q.
+Inductive derivable: 
+    nat -> nat -> 
+    Assertion 1 -> com -> Assertion 1 -> Type :=
+  | H_Skip : forall n (P: Assertion n),
+    derivable n n P <{ skip }> P
+  | H_App : forall n G (P: Assertion n) m,
+    derivable n n (apply_sub n m (geval G) P) <{ q m *= G }> P
+  | H_Init : forall n (P: Assertion n),
+    derivable (n - 1)%nat n (init_sub n P) <{ new_qubit }> P
+  | H_Asgn : forall n (P: Assertion n) x e,
+    derivable n n (AssertPreAsgn P x e) <{ x := e }> P
+  | H_Meas_0 : forall n m (P: Assertion n) x,
+    derivable n n (AssertPreMeas P x 0 m) <{ x :=meas m }> P
+  | H_Meas_1 : forall n m (P: Assertion n) x,
+    derivable n n (AssertPreMeas P x 1 m) <{ x :=meas m }> P
+  | H_Seq : forall np nq nr (P: Assertion np) c 
+                   (Q: Assertion nq) d (R: Assertion nr),
+    derivable np nq P c Q -> 
+    derivable nq nr Q d R -> 
+    derivable np nr P <{ c;d }> R
+  | H_If : forall np nq (P: Assertion np) 
+                  (Q: Assertion nq) b c1 c2,
+    derivable np nq (AssertPreIfTrue P b) c1 Q ->
+    derivable np nq (AssertPreIfTrue P (BNot b)) c2 Q ->
+    derivable np nq P <{if b then c1 else c2 end}> Q
+  | H_While : forall n (P: Assertion n) b c,
+    derivable n n (AssertPreIfTrue P b) c P ->
+    derivable n n P <{while b do c end}> (AssertPreIfTrue P (BNot b))
+  | H_Weakness : forall np nq np' nq' 
+         (P: Assertion np) (Q: Assertion nq) 
+         (P': Assertion np') (Q': Assertion nq') c,
+    derivable np nq P c Q ->
+    (forall ns (st: State ns), weaker ns np np' st P' P) ->
+    (forall ns (st: State ns), weaker ns nq nq' st Q Q') ->
+    derivable np' nq' P' c Q'.
 
-Definition valid (P : Assertion) (c : com) (Q : Assertion) : Prop :=
-  forall st st',
-     st =[ c ]=> st' ->
-     P st ->
-     Q st'.
+Definition valid {np nq} (P : Assertion np) (c : com) (Q : Assertion nq) 
+      : Prop :=
+  forall ns1 ns2  (st1: State ns1) (st2: State ns2), 
+  (ceval ns1 ns2 c st1 st2) ->
+  (Expectation ns1 np st1 P) <= (Expectation ns2 nq st2 Q).
 
-Theorem logic_sound : forall P c Q,
-  derivable P c Q -> valid P c Q.
+Theorem logic_sound : forall np nq (P: Assertion np) c (Q: Assertion nq),
+  derivable np nq P c Q -> valid P c Q.
 Proof.
+  intros.
+  case_eq X.
+  - intros. induction X; apply fy_skip.
+  - intros. induction X; apply fy_apply.
+  - intros. induction X; apply fy_init.
+  - intros. induction X; apply fy_assign.  
+  - intros. induction X; apply fy_measure.
+  - intros. induction X; apply fy_measure.
+  - intros. induction X. apply fy_sequence with nq0 Q0.
+    induction d0. apply fy_skip. apply fy_apply. 
+    apply fy_init. apply fy_assign. apply fy_measure. apply fy_measure.
 Admitted.
 
-Theorem hoare_complete: forall P c Q,
-  valid P c Q -> derivable P c Q.
+Theorem logic_complete: forall np nq (P: Assertion np) c (Q: Assertion nq),
+  valid P c Q -> derivable np nq P c Q.
 Proof.
 Admitted.
